src/Ex/Mesi/MesiInvB.v
@@ -1,0 +1,44 @@
+Require Import Bool List String Peano_dec Lia.
+Require Import Common FMap IndexSupport HVector Syntax Topology Semantics SemFacts StepM.
+Require Import Invariant TrsInv Simulation Serial SerialFacts.
+Require Import RqRsLang RqRsCorrect.
+
+Require Import Ex.Spec Ex.SpecInds Ex.Template.
+Require Import Ex.Mesi Ex.Mesi.Mesi Ex.Mesi.MesiTopo.
+
+Set Implicit Arguments.
+
+Import PropMonadNotations.
+Import CaseNotations.
+
+Local Open Scope list.
+Local Open Scope hvec.
+Local Open Scope fmap.
+
+Existing Instance Mesi.ImplOStateIfc.
+
+Section Footprints.
+  Variable topo: DTree.
+
+  Definition DownLockFromChild (oidx: IdxT) (rqid: RqInfo Msg) :=
+    exists cidx,
+      rqid.(rqi_midx_rsb) = Some (downTo cidx) /\
+      parentIdxOf topo cidx = Some oidx.
+
+  Definition DownLockFromParent (oidx: IdxT) (rqid: RqInfo Msg) :=
+    rqid.(rqi_midx_rsb) = Some (rqUpFrom oidx).
+
+  Definition MesiFootprintsInv (st: MState): Prop :=
+    forall oidx,
+      orq <+- (bst_orqs st)@[oidx];
+        rqid <+- orq@[downRq];
+        rmsg <+- rqid.(rqi_msg);
+        match case rmsg.(msg_id) on idx_dec default True with
+        | mesiRqS: DownLockFromChild oidx rqid
+        | mesiRqM: DownLockFromChild oidx rqid
+        | mesiDownRqS: DownLockFromParent oidx rqid
+        | mesiDownRqI: DownLockFromParent oidx rqid
+        end.
+
+End Footprints.
+
